facts and lemmas about shared keys

scripts/Smartphone.thy
@@ -6,18 +6,16 @@ Theory for offline and out-of-band channels, defined by communications
   means created using the smartphone camera for decoding QR codes displayed
   at other insecure devices screens.
 
-Definitions for keys, initial state of agents and smartphone's usability
+Definitions for keys, initial state of agents and smartphone's usability.
 *)
 
-theory Smartphone imports "./EventSP" begin
+theory Smartphone imports "./EventSP" "~~/src/HOL/Auth/All_Symmetric" begin
 
 axiomatization
-  shrK  ::  "agent \<Rightarrow> key" and
-  phnK  ::  "smartphone \<Rightarrow> key"
+  shrK  ::  "agent \<Rightarrow> key"
 
 where
-  inj_shrK : "inj shrK" and
-  inj_phnK : "ink phnK"
+  inj_shrK : "inj shrK"
 
 definition legalUse :: "smartphone \<Rightarrow> bool" ("legalUse (_)") where
   "legalUse P == P \<notin> stolen"
@@ -32,8 +30,49 @@ overloading initState \<equiv> initState
   primrec initState where
     initState_Server : "initState Server = (Key`(range shrK))" |
     initState_Friend : "initState (Friend i) = {Key (shrK(Friend i))}" |
-    initState_Spy : "initState Spy = (Key`(range shrK) \<union> (Key` phnK` (badp \<inter> connected)))"
-  end
+    initState_Spy : "initState Spy = (Key`((shrK` bad) \<union> (shrK`{A. Smartphone A \<in> (badp \<inter> connected)}) ))"
+end
+
+axiomatization where
+  Key_sypply_ax: "finite KK \<Longrightarrow> \<exists> K. K \<notin> KK & Key K \<notin> used evs "
+
+
+(* PROPERTIES OF SHARED KEYS *)
+declare inj_shrK [THEN inj_eq, iff]
+
+lemma invKey_K [simp]: "invKey K = K"
+apply (insert isSym_keys)
+apply (simp add: symKeys_def)
+done
+
+lemma analz_Decrypt' [dest]:
+  "\<lbrakk> Crypt K X \<in> analz H; Key K \<in> analz H \<rbrakk> \<Longrightarrow> X \<in> analz H"
+apply (auto)
+done
+declare analz.Decrypt [rule del]
+
+lemma parts_image_Nonce [simp]: "parts (Nonce`N) = Nonce`N"
+apply (auto)
+done
+
+lemma keysFor_parts_initState [simp] : 
+  "keysFor (parts (initState C)) = {}"
+apply (unfold keysFor_def)
+apply (induct_tac "C", auto)
+done
+
+(* IF a key K is present in the set of useful keys to decrypt message X in a given message set G
+ and  message X can be constructed given analysis of a message set H,
+ THEN key K must be either in set G or H  *)
+lemma keysFor_parts_insert : 
+  "\<lbrakk> K \<in> keysFor (parts (insert X G)); X \<in> synth (analz H) \<rbrakk>
+    \<Longrightarrow> K \<in> keysFor (parts (G \<union> H)) | Key K \<in> parts H"
+by (force dest: EventSP.keysFor_parts_insert)
+
+
+lemma Crypt_imp_keysFor : 
+  "Crypt K X \<in> H \<Longrightarrow> K \<in> keysFor H"
+by (drule Crypt_imp_invKey_keysFor, simp)
 
 
 end
